\documentclass[12pt, a4paper]{article}

\usepackage{amsmath}
\usepackage{graphicx}
\usepackage{float}
\usepackage{listings}
\usepackage{color}

\lstset{
	numbers=left, 
	numberstyle=\small, 
	numbersep=8pt, 
	frame = single, 
	language=Python, 
	framexleftmargin=15pt,
	breaklines,
	showspaces=false, 
	showstringspaces=false, 
	backgroundcolor=\color{white}, 
	keywordstyle=\color{red}\bfseries, 
	showtabs=false} 

\usepackage[norsk]{babel}
\usepackage{csquotes}
\usepackage{todonotes} 
\usepackage{subcaption}
\usepackage{comment}
\usepackage{wrapfig}
\usepackage[margin=0.7in]{geometry}

\title{Wave Project - Finite difference simulation of 2D waves}
\date{October 2019}
\author{Marte Fossum}

\begin{document}

\maketitle
\newpage

{\setlength{\parindent}{0cm}

\section*{Discretization}

We are give the equation 

\begin{align}
    \frac{\partial^{2} u}{\partial t^{2}}+b \frac{\partial u}{\partial t}=\frac{\partial}{\partial x}\left(q(x, y) \frac{\partial u}{\partial x}\right)+\frac{\partial}{\partial y}\left(q(x, y) \frac{\partial u}{\partial y}\right)+f(x, y, t)
    \label{maineq}
\end{align} 

with the boundary condition

\begin{align*}
    \frac{\partial u}{\partial n} = 0
\end{align*}

on the domain \(\Omega = [0, L_x] \times [0, L_y]\), with initial conditions 

\begin{align}\label{icu}
    u(x, y, 0) =I(x, y) 
\end{align}
\begin{align}\label{icuder}
    u_{t}(x, y, 0) =V(x, y) 
\end{align}

We want to discretize equation (\ref{maineq}) in order to simulate it on the computer. By letting \(u(x_i, y_j, t_n) = u_{i, j}^n\) we can rewrite each term as

\begin{align*}
    \frac{\partial^2 u}{\partial t^2} &= \frac{u_{i,j}^{n+1} - 2u_{i,j}^n + u_{i,j}^{n-1}}{\Delta t^2} \\\\ 
    b\frac{\partial u}{\partial t} &= b\frac{u_{i,j}^{n+1}- u_{i,j}^{n-1}}{2\Delta t} \\\\
    \frac{\partial}{\partial x}\left(q(x, y) \frac{\partial u}{\partial x}\right) &= \frac{\frac{1}{2}(q_{i,j} + q_{i+1,j})(u_{i+1,j}^n - u_{i,j}^n) - \frac{1}{2}(q_{i,j} + q_{i-1,j})(u_{i,j}^{n} - u_{i-1,j}^{n})}{\Delta x^2} \\\\
    \frac{\partial}{\partial y}\left(q(x, y) \frac{\partial u}{\partial y}\right) &= \frac{\frac{1}{2}(q_{i,j} + q_{i,j+1})(u_{i,j+1}^n - u_{i,j}^n) - \frac{1}{2}(q_{i,j} + q_{i,j-1})(u_{i,j}^{n} - u_{i,j-1}^{n})}{\Delta y^2} \\\\
    f(x, y, t) &= f(x_i, y_j, t_n) \\\\
\end{align*}

Inserting this into (\ref{maineq}) gives us

\begin{equation}\label{mainnum}
\begin{aligned}
    \frac{u_{i,j}^{n+1} - 2u_{i,j}^n + u_{i,j}^{n-1}}{\Delta t^2} + b\frac{u_{i,j}^{n+1}- u_{i,j}^{n-1}}{2\Delta t} = &\frac{\frac{1}{2}(q_{i,j} + q_{i+1,j})(u_{i+1,j}^n - u_{i,j}^n) - \frac{1}{2}(q_{i,j} + q_{i-1,j})(u_{i,j}^{n} - u_{i-1,j}^{n})}{\Delta x^2} \\ &+ \frac{\frac{1}{2}(q_{i,j} + q_{i,j+1})(u_{i,j+1}^n - u_{i,j}^n) - \frac{1}{2}(q_{i,j} + q_{i,j-1})(u_{i,j}^{n} - u_{i,j-1}^{n})}{\Delta y^2} \\ &+ f(x_i, y_j, t_n)
\end{aligned}
\end{equation}

Now we solve for \(u_{i,j}^{n+1}\).

\begin{equation}\label{un} 
\begin{aligned}
    u_{i,j}^{n+1} = &\left(\frac{\Delta t^2}{1 + \frac{\Delta tb}{2}}\right)\left(\frac{\frac{1}{2}(q_{i,j} + q_{i+1,j})(u_{i+1,j}^n - u_{i,j}^n) - \frac{1}{2}(q_{i,j} + q_{i-1,j})(u_{i,j}^{n} - u_{i-1,j}^{n})}{\Delta x^2}\right) \\ &+ \left(\frac{\Delta t^2}{1 + \frac{\Delta tb}{2}}\right)\left(\frac{\frac{1}{2}(q_{i,j} + q_{i,j+1})(u_{i,j+1}^n - u_{i,j}^n) - \frac{1}{2}(q_{i,j} + q_{i,j-1})(u_{i,j}^{n} - u_{i,j-1}^{n})}{\Delta y^2}\right) \\ &+ \left(\frac{1}{1 + \frac{\Delta tb}{2}}\right)\left(\Delta t^2 f(x_i, y_j, t_n) + 2u_{i,j}^n + u_{i,j}^{n-1}\left(\frac{\Delta tb}{2} - 1\right)\right)\\\\
\end{aligned}       
\end{equation}      

In order for us to use this equation, we have to know the first time step. To get \(u^1\) we use the initial conditions (\ref{icu}) and (\ref{icuder}). From (\ref{icu}) we get that \(u^0 = I(x, y)\) and by discretizing (\ref{icuder}) we get that 

\begin{equation*}
\begin{aligned}
    \frac{u^1 - u^{-1}}{2 \Delta t} = V 
    \implies u^{-1} = u^1 - 2V \Delta t
\end{aligned}    
\end{equation*}

We set \(n = 0\) and set in for \(u^{-1}\) and solve for \(u^1\). This gives us

\section*{Vertification}

We now assume that \(u(x, y, t) = C\) where \(C\) is a constant. We want to show that the constant solution is a solution of the descrete equation also.

\begin{equation*}
\begin{aligned}
    \frac{u_{i,j}^{n+1} - 2u_{i,j}^n + u_{i,j}^{n-1}}{\Delta t^2} &= \frac{C - 2C + C}{\Delta t^2} = 0 \\\\
    b\frac{u_{i,j}^{n+1}- u_{i,j}^{n-1}}{2\Delta t} &= b\frac{C - C}{2\Delta t}
    = 0 \\\\
    \frac{q_{1 + \frac{1}{2}}(u_{i+1,j}^n - u_{i,j}^n) - q_{1 - \frac{1}{2}}(u_{i,j}^{n} - u_{i-1,j}^{n})}{\Delta x^2} &= \frac{q_{1 + \frac{1}{2}}(C - C) - q_{1 - \frac{1}{2}}(C - C)}{\Delta x^2}
    = 0 \\\\
    \frac{q_{1 + \frac{1}{2}}(u_{i+1,j}^n - u_{i,j}^n) - q_{1 - \frac{1}{2}}(u_{i,j}^{n} - u_{i-1,j}^{n})}{\Delta y^2} &= \frac{q_{1 + \frac{1}{2}}(C - C) - q_{1 - \frac{1}{2}}(C - C)}{\Delta y^2}
    = 0
\end{aligned}
\end{equation*}

So the constant solution is a solution for the discrete equations when \(f(x, y, t) = 0\) and the initial conditions are \(u(x, y, 0) = C\) and \(u_t(x, y, t) = 0\).

\subsection*{5 possible bugs}

\begin{itemize}
    \item 1
    \item 2
    \item 3
    \item 4
    \item 5
\end{itemize}

\section*{}
\end{document} 